Continue pruning itree. Now we need to actually run the region.
run (interp (denoteOp_interp_region scf (denoteRegions scf [r])) (run_loop_bounded (n + 1) 0 (BlockResult.Ret [])))
    (INPUT n) =
  match run (List.get! (denoteRegions scf [r]) 0 [{ fst := MLIRType.index, snd := 0 }]) (INPUT n) with
  | (none, env') => (none, env')
  | (some x, env') =>
    run
      (Fitree.Vis (Sum.inr (Sum.inl (SSAEnvE.Get MLIRType.index (SSAVal.SSAVal "c1")))) fun r_1 =>
        Fitree.Vis (Sum.inr (Sum.inl (SSAEnvE.Get MLIRType.index (SSAVal.SSAVal "cn_plus_1")))) fun r_2 =>
          interp (denoteOp_interp_region scf (denoteRegions scf [r]))
            (run_loop_bounded (r_2 - r_1) 0 (BlockResult.Ret [])))
      env'

MLIR/Semantics/Semantics.lean
@@ -96,7 +96,7 @@ class Semantics (δ: Dialect α σ ε)  where
 mutual
 variable (Δ: Dialect α' σ' ε') [S: Semantics Δ]
 
-def interp_region
+def denoteOp_interp_region
     (regions: List <|
       TypedArgs Δ → Fitree (UBE +' SSAEnvE Δ +' S.E) (BlockResult Δ)):
     RegionE Δ +' UBE +' Semantics.E Δ ~>
@@ -123,7 +123,7 @@ def denoteOp (op: Op Δ):
       -- Use the dialect-provided semantics, and substitute regions
       match S.semantics_op iop with
       | some t =>
-          interp (interp_region regions) t
+          interp (denoteOp_interp_region regions) t
       | none => do
           Fitree.trigger <| UBE.DebugUB s!"invalid op: {op}"
           return default
